# 3.4

$$
x_{n+1} = x_n = x^*
$$

代入差分方程：

$$
x^* = 4x^*(3 - x^*)
$$

得到两个平衡点：

$$
x^* = 0 \quad \text{或} \quad x^* = \frac{11}{4}
$$


# 5

## 1

$$
\begin{align*}
P_{2005} &= rP_{2000} \Rightarrow 2352 = r \cdot 2104 \Rightarrow r = \frac{2352}{2104} \approx 1.118 {\color{gray}} \\
P_{2010} &= rP_{2005} \Rightarrow 2573 = r \cdot 2352 \Rightarrow r = \frac{2573}{2352} \approx 1.094 {\color{gray}} \\
P_{2015} &= rP_{2010} \Rightarrow 3123 = r \cdot 2573 \Rightarrow r = \frac{3123}{2573} \approx 1.214 {\color{gray}} \\
P_{2020} &= rP_{2015} \Rightarrow 3824 = r \cdot 3123 \Rightarrow r = \frac{3824}{3123} \approx 1.225 {\color{gray}} \\
\end{align*}
$$


$$
r \approx \frac{1.118 + 1.094 + 1.214 + 1.225}{4} = \frac{4.651}{4} \approx 1.16
$$

所以参数为：

- $P_{2000} = 2104$
- $r = 1.16$

---

## 2


$$
P(n) = \sum_{i=0}^4 P(x_i) \cdot L_i(n)
$$

其中：

$$
L_i(n) = \prod_{\substack{j=0 \\ j\ne i}}^4 \frac{n - x_j}{x_i - x_j}
$$

所以表达式是：

$$
\begin{aligned}
P(n) = & \; 2104 \cdot \frac{(n - 2005)(n - 2010)(n - 2015)(n - 2020)}{(2000 - 2005)(2000 - 2010)(2000 - 2015)(2000 - 2020)} \\
&+ 2352 \cdot \frac{(n - 2000)(n - 2010)(n - 2015)(n - 2020)}{(2005 - 2000)(2005 - 2010)(2005 - 2015)(2005 - 2020)} \\
&+ 2573 \cdot \frac{(n - 2000)(n - 2005)(n - 2015)(n - 2020)}{(2010 - 2000)(2010 - 2005)(2010 - 2015)(2010 - 2020)} \\
&+ 3123 \cdot \frac{(n - 2000)(n - 2005)(n - 2010)(n - 2020)}{(2015 - 2000)(2015 - 2005)(2015 - 2010)(2015 - 2020)} \\
&+ 3824 \cdot \frac{(n - 2000)(n - 2005)(n - 2010)(n - 2015)}{(2020 - 2000)(2020 - 2005)(2020 - 2010)(2020 - 2015)} \\
\end{aligned}
$$
